wip

fstar-helpers/fstar-bitvec/RwLemmas.fst
@@ -11,6 +11,7 @@ open FStar.Option
 open Tactics.Utils
 open Tactics.Pow2
 
+open BitVecEq {}
 
 let norm_machine_int () = Tactics.MachineInts.(transform norm_machine_int_term)
 
@@ -64,7 +65,7 @@ let split_forall_nat
 
 // #push-options "--z3rlimit 60"
 let rw_bit_or (b1 b2: bit) result:
-  Lemma 
+  Lemma
     (requires (
         (b1 = 0 ==> b2 = 0 ==> result = 0)
       /\ (b1 = 0 ==> b2 = 1 ==> result = 1)
@@ -108,10 +109,12 @@ let rw_get_bit_and (x y: int_t 't) i
 let rw_get_bit_and_left (x y: int_t 't) i
   : Lemma (requires get_bit x i == 0) 
           (ensures get_bit (x &. y) i == 0)
+          [SMTPat (get_bit (x &. y) i)]
   = get_bit_and x y i
 let rw_get_bit_and_right (x y: int_t 't) i
   : Lemma (requires get_bit x i == 0) 
           (ensures get_bit (y &. x) i == 0)
+          [SMTPat (get_bit (y &. x) i)]
   = get_bit_and x y i
 let rw_get_bit_or_left (x y: int_t 't) i
   : Lemma (requires get_bit x i == 0)
@@ -162,10 +165,6 @@ let pow2_in_range t (n: nat {n < bits t - (if unsigned t then 0 else 1)})
       [SMTPat (Rust_primitives.Integers.range (pow2 n - 1) t)]
     = Math.Lemmas.pow2_le_compat (bits t - (if unsigned t then 0 else 1)) n
 
-exception Restore
-let dump' (msg: string): Tac unit
-    = try let _ = repeat clear_top in set_smt_goals []; dump msg with | _ -> ()
-
 // let _ = op_Bar_Dot
 
 noeq type bit_expr =
@@ -177,9 +176,61 @@ noeq type bit_expr =
   | Shr: x:bit_expr -> shift:int -> bit_expr
   | Cast: x:bit_expr -> bit_expr
 
+let rec term_eq'' a b (n: nat): Tot _ (decreases n) =
+  let open FStar.Stubs.Reflection.V2.Data in
+  if n = 0 then term_eq a b else
+  match (inspect_ln a, inspect_ln b) with
+  | (Tv_FVar a, Tv_FVar b)
+  | (Tv_FVar a, Tv_UInst b _)
+  | (Tv_UInst a _, Tv_FVar b)
+  | (Tv_UInst a _, Tv_UInst b _) -> inspect_fv a = inspect_fv b
+  | (Tv_Var _, Tv_Var _) -> term_eq a b
+  | (Tv_App _ _, Tv_App _ _) ->
+    let a, a_args = collect_app_ln a in
+    let b, b_args = collect_app_ln b in
+    let a_args = L.filter (fun (_, x) -> Q_Explicit? x) a_args in
+    let b_args = L.filter (fun (_, x) -> Q_Explicit? x) b_args in
+    L.length a_args = L.length b_args
+    && (
+    let rec h a_args (b_args: _ {L.length a_args == L.length b_args}) =
+      match a_args, b_args with
+      | ((ahd,_)::atl), ((bhd,_)::btl) -> 
+        term_eq'' ahd bhd (n - 1) && h atl btl
+      | [], [] -> true
+    in h a_args b_args
+    )
+  | (Tv_AscribedT a _ _ _, _)
+  | (Tv_AscribedC a _ _ _, _) -> term_eq'' a b (n-1)
+  | (_, Tv_AscribedT b _ _ _)
+  | (_, Tv_AscribedC b _ _ _) -> term_eq'' a b (n-1)
+  | (Tv_Type _, Tv_Type _) -> true
+  | (Tv_Refine _ a, _) -> term_eq'' a b (n - 1)
+  | (_, Tv_Refine _ b) -> term_eq'' a b (n - 1)
+    // && term_eq' a b && L.fold_left (fun i a -> L.index b_args i `term_eq'` a)
+  // | Tv_Var    : v:namedv -> named_term_view
+  // | Tv_BVar   : v:bv -> named_term_view
+  // | Tv_FVar   : v:fv -> named_term_view
+  // | Tv_UInst  : v:fv -> us:universes -> named_term_view
+  // | Tv_App    : hd:term -> a:argv -> named_term_view
+  // | Tv_Abs    : b:binder -> body:term -> named_term_view
+  // | Tv_Arrow  : b:binder -> c:comp -> named_term_view
+  // | Tv_Type   : universe -> named_term_view
+  // | Tv_Refine : b:simple_binder -> ref:term -> named_term_view
+  // | Tv_Const  : vconst -> named_term_view
+  // | Tv_Uvar   : nat -> ctx_uvar_and_subst -> named_term_view
+  // | Tv_Let    : recf:bool -> attrs:(list term) -> b:simple_binder -> def:term -> body:term -> named_term_view
+  // | Tv_Match  : scrutinee:term -> ret:option match_returns_ascription -> brs:(list branch) -> named_term_view
+  // | Tv_AscribedT : e:term -> t:term -> tac:option term -> use_eq:bool -> named_term_view
+  // | Tv_AscribedC : e:term -> c:comp -> tac:option term -> use_eq:bool -> named_term_view
+  // | Tv_Unknown  : named_term_view // An underscore: _
+  // | Tv_Unsupp : named_term_view // failed to inspect, not supported
+  | _ -> term_eq a b
+
+let term_eq' a b = term_eq'' a b 99999
+
 let rec bit_expr_eq a b =
   match (a, b) with
-  | Term a, Term b -> term_eq a b
+  | Term a, Term b -> term_eq' a b
   | Int a, Int b -> a = b
   | And xa ya, And xb yb
   | Or  xa ya, Or  xb yb -> bit_expr_eq xa xb && bit_expr_eq ya yb
@@ -238,14 +289,6 @@ let expect_get_bit_expr t: Tac _
     let expr = term_to_bit_expr' expr in
     Some (expr, index)
 
-let fail' msg = dump msg; fail msg
-
-let expect (msg: string) (x: option 'a): Tac 'a
-  = match x with
-  | None -> 
-    dump' ("Expected " ^ msg);
-    fail ("Expected " ^ msg)
-  | Some x -> x
 
 let op_Bar_GreaterThan (x: 'a) (f: 'a -> Tac 'b): Tac 'b = f x
 
@@ -255,7 +298,7 @@ let get_bit_shl_zero #t #u (x: int_t t) (y: int_t u) (i: usize {v i < bits t})
     = get_bit_shl x y i
 
 let get_bit_shr_zero #t #u (x: int_t t) (y: int_t u) (i: usize {v i < bits t})
-  : Lemma (requires v y >= 0 /\ v y < bits t /\ v i >= bits t - v y /\ (if signed t then (get_bit x (mk_int (bits t - 1)) == 0) else true))
+  : Lemma (requires v y >= 0 /\ v y < bits t /\ (v i >= bits t - v y /\ (if signed t then (get_bit x (mk_int (bits t - 1)) == 0) else true)))
           (ensures get_bit (x >>! y) i == 0)
     = get_bit_shr x y i
 
@@ -264,10 +307,22 @@ let get_bit_shl_one #t #u (x: int_t t) (y: int_t u) (i: usize {v i < bits t})
           (ensures get_bit (x <<! y) i == get_bit x (mk_int (v i - v y)))
     [SMTPat (get_bit (x <<! y) i)] = get_bit_shl x y i
 
-let rewrite_lhs (): Tac _ =
-  let (lhs, _, _) = expect_lhs_eq_rhs () |> expect "a goal `<lhs> == <rhs>` (rewrite_lhs)" in
-  let uvar = fresh_uvar (Some (tc (cur_env ()) lhs)) in
-  tcut (`squash (`#lhs == `#uvar))
+let get_bit_shr #t #u (x: int_t t) (y: int_t u {v y >= 0 /\ v y < bits t}) (i: usize {v i < bits t})
+  : Lemma (ensures get_bit (shift_right x y) i 
+               == 1)
+                // == (if v i < bits t - v y
+                //     then get_bit x (mk_int (v i + v y))
+                //     else if signed t
+                //          then get_bit x (mk_int (bits t - 1))
+                //          else 0))
+          // (ensures get_bit (x >>! y) i 
+          //       == (if v i < bits t - v y
+          //           then get_bit x (mk_int (v i + v y))
+          //           else if signed t
+          //                then get_bit x (mk_int (bits t - 1))
+          //                else 0))
+    [SMTPat (get_bit (x >>! y) i)]
+    = admit ()
 
 /// Proves that `get_bit .. ..` is zero
 let rec solve_get_bit_zero (): Tac _ =
@@ -280,12 +335,16 @@ let rec solve_get_bit_zero (): Tac _ =
   | Term _ -> fail ("LHS is an arbitrary term, I cannot prove it is " ^ string_of_int rhs')
   | Int _ -> (compute (); trefl ())
   | Shl _ _ -> 
-    apply_lemma (`get_bit_shl_zero);
+    let _ = rewrite_lhs () in
+    flip ();
+    apply_lemma_rw (`get_bit_shl);
     (fun _ -> 
     norm_machine_int (); compute (); norm [simplify];
     trivial () )`or_else` (fun _ -> fail' "Shl: tried to prove it was zero")
   | Shr _ _ -> 
-    apply_lemma (`get_bit_shr_zero);
+    let _ = rewrite_lhs () in
+    flip ();
+    apply_lemma_rw_eqtype (`get_bit_shr);
     focus (fun _ -> 
       let _ = repeat split in
       iterAll (fun _ -> 
@@ -338,7 +397,9 @@ let _solve_get_bit_equality lhs i rhs j: Tac _ =
         | true, false -> 
           let rw = rewrite_lhs () in
           flip ();
+          dump' "solve_get_bit_equality: LEFT (BEFORE)";
           apply_lemma_rw (norm_term [] (`rw_get_bit_or_right));
+          dump' "solve_get_bit_equality: LEFT (AFTE RLEMMA)";
           print "solve_get_bit_equality: LEFT";
           solve_get_bit_zero ()
         | false, true -> 
@@ -350,53 +411,94 @@ let _solve_get_bit_equality lhs i rhs j: Tac _ =
         )
   | _ -> fail' "xxxpppppp"
 
-let solve_get_bit_equality (): Tac _ =
+let swap_eq2_goal p q: Lemma (requires eq2 p q) (ensures eq2 q p) = ()
+
+let rec solve_get_bit_equality' can_invert: Tac _ =
   let (lhs, rhs, _) = expect_lhs_eq_rhs () |> expect "a goal `<lhs> == <rhs>`" in
   print ("solve_get_bit_equality: (" ^ term_to_string lhs ^ ") == (" ^ term_to_string rhs ^ ")");
   let (lhs, i) = expect_get_bit_expr lhs |> expect "LHS to be `get_bit .. ..`" in
   let (rhs, j) = expect_get_bit_expr rhs |> expect "RHS to be `get_bit .. ..`" in
   if bit_expr_contains rhs lhs |> not 
-  then fail "was expected the bit expression on RHS to be included in the one of LHS";
-  _solve_get_bit_equality lhs i rhs j;
-  ()
+  then if can_invert
+       then (apply_lemma (`swap_eq2_goal); solve_get_bit_equality' false)
+       else fail "was expected the bit expression on RHS to be included in the one of LHS"
+  else _solve_get_bit_equality lhs i rhs j
+let solve_get_bit_equality (): Tac _ =
+  solve_get_bit_equality' true
 
+let rec term_to_string'' (t: term): Tac string
+  = match t with
+  | Tv_App f (x, Q_Meta _) -> term_to_string'' f
+  | Tv_App f (x, aqualv) ->
+    let qual = match aqualv with | Q_Implicit -> "#" | Q_Explicit -> "" in
+    term_to_string' f ^ " " ^ qual ^ "(" ^ term_to_string' x ^ ")"
+  | Tv_UInst v _ | Tv_FVar v -> 
+      let v = implode_qn (inspect_fv v) in
+      (match v with
+      | `%get_bit -> "get_bit"
+      | `%bit -> "bit"
+      | `%eq2 -> "eq2"
+      | `%u8 -> "u8"
+      | `%u16 -> "u16"
+      | `%i16 -> "i16"
+      | `%i32 -> "i32"
+      | `%sz -> "sz"
+      | `%usize -> "usize"
+      | _ -> v
+      )
+  | _ -> term_to_string t
+and term_to_string' t: Tac _ =  term_to_string'' t
+
+// get_bit (Seq.Base.index bytes 2) (sz 1) ==
+// get_bit ((cast bytes.[ sz 2 ] &. 15s) <<! 6l |. cast bytes.[ sz 1 ] >>! 2l) (sz 7)
+
+let opts = "--using_facts_from '-* +Rust_primitives.BitVectors
++Rust_primitives.Integers.get_bit_cast +Rust_primitives.Integers.get_bit_and +Rust_primitives.Integers.get_bit_or +Rust_primitives.Integers.get_bit_shl +Rust_primitives.Integers.get_bit_shr +Rust_primitives.Integers.get_bit_cast_extend'"
+
+#push-options "--z3rlimit 80"
+let fff_ bytes x: unit = 
+    let bv1 = bit_vec_of_int_t_array bytes 8 in
+    let out = deserialize_10_int' bytes in
+    let bv2 = bit_vec_of_int_t_array out 10 in
+    let i = 77 in
+    if false then
+    assert (bv1 i == bv2 i) by (
+      norm [
+        iota; primops; 
+        delta_only [`%bit_vec_of_int_t_array; `%FunctionalExtensionality.on];
+      ];
+      compute'' ();
+      set_options opts;
+      dump "SMT NOW";
+      smt_sync ();
+      // squash_intro ();
+      // print (term_to_string' (cur_goal()));
+      fail "DONE"
+    )
+#pop-options
 
 #push-options "--compat_pre_core 0"
+#push-options "--z3rlimit 80"
+#push-options "--print_implicits"
 let asdsd (bytes: t_Array u8 (sz 10))
     = let cast: u8 -> i16 = cast in
       assert (
-         get_bit (
-              ((cast bytes.[ sz 3 ] <: i16) &. 63s <: i16) <<! 4l 
-           |. (cast bytes.[ sz 2 ] <: i16) >>! 4l
-         ) (sz 5)
-         == get_bit (cast bytes.[ sz 3 ] <: i16) (sz 0)
+        eq2 #(bit) (get_bit #(Lib.IntTypes.U8) (FStar.Seq.Base.index #(Rust_primitives.Integers.int_t (Lib.IntTypes.U8)) (bytes) (2)) (sz (1))) (get_bit #(Lib.IntTypes.S16) (Rust_primitives.Integers.op_Bar_Dot #(Lib.IntTypes.S16) (Rust_primitives.Integers.op_Less_Less_Bang #(Lib.IntTypes.S16) #(Lib.IntTypes.S32) (Rust_primitives.Integers.op_Amp_Dot #(Lib.IntTypes.S16) (Rust_primitives.cast #(u8) #(i16) #(Rust_primitives.cast_tc_integers (Lib.IntTypes.U8) (Lib.IntTypes.S16)) (Core.Ops.op_String_Access #(Rust_primitives.Arrays.t_Array (u8) (sz (10))) #(usize) #(Rust_primitives.Hax.impl__index (u8) (sz (10)) (Rust_primitives.Integers.usize_inttype)) (bytes) (sz (2)))) (FStar.Int16.int_to_t (15))) (FStar.Int32.int_to_t (6))) (Rust_primitives.Integers.op_Greater_Greater_Bang #(Lib.IntTypes.S16) #(Lib.IntTypes.S32) (Rust_primitives.cast #(u8) #(i16) #(Rust_primitives.cast_tc_integers (Lib.IntTypes.U8) (Lib.IntTypes.S16)) (Core.Ops.op_String_Access #(Rust_primitives.Arrays.t_Array (u8) (sz (10))) #(usize) #(Rust_primitives.Hax.impl__index (u8) (sz (10)) (Rust_primitives.Integers.usize_inttype)) (bytes) (sz (1)))) (FStar.Int32.int_to_t (2)))) (sz (7)))
+         // get_bit (
+         //      ((cast bytes.[ sz 3 ] <: i16) &. 63s <: i16) <<! 4l 
+         //   |. (cast bytes.[ sz 2 ] <: i16) >>! 4l
+         // ) (sz 5)
+         // == get_bit (cast bytes.[ sz 3 ] <: i16) (sz 0)
       ) by (
+        norm [iota; delta_only [`%( .[] ); `%Core.Ops.Index.Mkt_Index; `%Rust_primitives.Hax.impl__index; `%Core.Ops.Index.f_index]];
         Tactics.MachineInts.(transform norm_generic_machine_int_term);
         solve_get_bit_equality ();
-        // dump "XXXX";
-        // simplify_via_mask ();
-        // fail "-------";
-        // pointwise' (fun _ -> 
-        //    let _ = let?# (t, _) = expect_lhs_eq_uvar () in
-                   
-        //            let?# (f, _) = expect_app_n t 3 in
-        //            let?# () = expect_free_var f (`%get_bit) in
-        //            // norm [ iota; zeta; reify_
-        //            //      ; primops; unmeta];
-        //            dump' "xxxxx";
-        //            // apply_lemma_rw (`(rw_rhs_bit_or_no_mask #Lib.IntTypes.U8 #Lib.IntTypes.S16 #Lib.IntTypes.S32 ((`@cast) (`@bytes).[ sz 3 ] &. 63s <: i16)));
-        //            // invert ();
-        //            Some ()
-        //    in
-        //    trefl ()
-        //    // let _ = repeat clear_top in
-        //    // dump "X";
-        //    // (fun _ -> apply_lemma_rw (`rw_rhs_bit_or_no_mask)) `or_else` trefl;
-        //    // let _ = repeat clear_top in
-        //    // dump "Y"
-        // );
+        // print (term_to_string' (cur_goal()));
+        // smt_sync ();
         fail "done"
       )
+
+
 
 
 
