fstar-helpers/fstar-bitvec/Tactics.Utils.fst
@@ -32,12 +32,15 @@ let expect_free_var (t: term) (fv: string): Tac (option unit) =
     let?# fv' = expect_fvar t in
     if fv = fv' then Some () else None
 
-let expect_lhs_eq_rhs () = 
-    match FStar.Tactics.V2.Logic.cur_formula () with
+let expect_lhs_eq_rhs_term t = 
+    match term_as_formula t with
     | Comp (Eq typ) lhs rhs -> 
       let typ = match typ with | None -> `_ | Some typ -> typ in
       Some (lhs, rhs, typ)
     | _ -> None
+
+let expect_lhs_eq_rhs () = 
+    expect_lhs_eq_rhs_term (cur_goal ())
 
 let expect_lhs_eq_uvar () = 
     match expect_lhs_eq_rhs () with
@@ -65,3 +68,73 @@ let collect_app_hd t: Tac (option (string & list argv))
 
 let rec repeatWhile (f: unit -> Tac bool): Tac unit
   = if f () then repeatWhile f
+
+
+let fail' msg = dump msg; fail msg
+
+exception Restore
+let dump' (msg: string): Tac unit
+    = try set_smt_goals [];
+          iterAll (fun _ -> let _ = repeat clear_top in ());
+          dump msg;
+          raise Restore
+      with | _ -> ()
+
+let expect (msg: string) (x: option 'a): Tac 'a
+  = match x with
+  | None -> 
+    dump' ("Expected " ^ msg);
+    fail ("Expected " ^ msg)
+  | Some x -> x
+
+
+let statement_of_lemma (lemma: term) =
+  let _, comp = collect_arr (tc (cur_env ()) lemma) in
+  match inspect_comp comp with
+  | C_Total x
+  | C_Lemma _ x _ -> (
+      match x with
+      | Tv_Abs _ x -> `(squash (`#x))
+      | _ -> `(squash (`#x))
+    )
+  | _ -> fail "statement_of_lemma: supports only Tot and Lemma"
+
+let weaken_eq2_lemma (u: Type) (t: Type {subtype_of t u}) (p q: t) ()
+  : Lemma (requires ( == ) #u p q)
+          (ensures  ( == ) #t p q)
+  = ()
+  
+let apply_lemma_rw_eqtype (lemma: term): Tac unit
+  = try
+      apply_lemma_rw lemma 
+    with
+    | e -> match
+            let stmt = statement_of_lemma lemma in
+            let?# (lemma_lhs, lemma_rhs, type_lemma') = expect_lhs_eq_rhs_term stmt in
+            let?# (goal_lhs, goal_rhs, type_goal') = expect_lhs_eq_rhs () in
+            let type_lemma = norm_term [delta; iota; primops] type_lemma' in
+            let type_goal  = norm_term [delta; iota; primops] type_goal'  in
+            if term_eq type_lemma type_goal
+            then None
+            else
+              ( print "######## Warning: apply_lemma_rw, rewrite equalities with different type";
+                print ("######## Your lemma has eq over type " ^ term_to_string type_lemma);
+                print ("######## Your goal has eq over type " ^ term_to_string type_goal);
+                print ("######## Trying to weaken the type of the goal.");
+                apply_lemma (
+                  `weaken_eq2_lemma
+                    (`#type_lemma') (`#type_goal')
+                    (`#goal_lhs) (`#goal_rhs)
+                );
+                apply_lemma_rw lemma;
+                Some ()
+              )
+          with | None -> raise e
+               | Some () -> ()
+
+
+let rewrite_lhs (): Tac _ =
+  let (lhs, _, _) = expect_lhs_eq_rhs () |> expect "a goal `<lhs> == <rhs>` (rewrite_lhs)" in
+  let uvar = fresh_uvar (Some (tc (cur_env ()) lhs)) in
+  tcut (`squash (`#lhs == `#uvar))
+  
